examples/wysteria/ast.fst
@@ -19,28 +19,22 @@ let p_cmp p1 p2 = p1 <= p2
 
 type prins = ordset prin p_cmp
 
-(* TODO:FIXME: hack, we don't have s1 = s2 ==> subset s1 s2 yet *)
 val subset: prins -> prins -> Tot bool
-let subset ps1 ps2 = (ps1 = ps2) || OrdSet.subset p_cmp ps1 ps2
+let subset = OrdSet.subset p_cmp
 
-assume val subset_transitive: ps1:prins -> ps2:prins -> ps3:prins
-                              -> Lemma (requires (subset ps1 ps2 /\ subset ps2 ps3))
-                                       (ensures  (subset ps1 ps3))
-                                 [SMTPat (subset ps1 ps2); SMTPat (subset ps2 ps3)]
-                                 
 val mem: prin -> prins -> Tot bool
 let mem = OrdSet.mem p_cmp
 
 assume val mem_subset: p:prin -> ps1:prins -> ps2:prins
-                       -> Lemma (requires (mem p ps1 /\ subset ps1 ps2))
-                                (ensures  (mem p ps2))
-                          [SMTPat (subset ps1 ps2)]
+                              -> Lemma (requires (mem p ps1 /\ subset ps1 ps2))
+                                       (ensures  (mem p ps2))
+                                [SMTPat (subset ps1 ps2)]
 
-val singleton: prin -> Tot (ps:prins{OrdSet.size p_cmp ps = 1})
-let singleton p = OrdSet.singleton p_cmp p
+val singleton: prin -> Tot prins
+let singleton = OrdSet.singleton p_cmp
 
 val is_singleton: prins -> Tot bool
-let is_singleton ps = (OrdSet.size p_cmp ps = 1)
+let is_singleton = OrdSet.is_singleton p_cmp
 
 assume val mem_subset_singleton:
   p:prin -> ps:prins
@@ -58,8 +52,7 @@ type const =
 
 type exp' =
   | E_aspar: ps:exp -> e:exp -> exp'
-  (*| E_assec: ps:exp -> e:exp -> exp'*)
-  | E_unbox: e:exp -> exp'
+  | E_unbox: e:exp  -> exp'
 
   | E_const: c:const -> exp'
   | E_var  : x:varname -> exp'
@@ -90,29 +83,23 @@ type redex =
 
 assume val empty_env: env
 
-val to_exp: exp' -> Tot exp
-let to_exp e = Exp e None
-
 val update_env: env -> varname -> value -> Tot env
 let update_env en x v = fun y -> if y = x then v else en y
 
 type as_mode =
   | Par
-  (*| Sec*)
 
 type mode =
   | Mode: m:as_mode -> ps:prins -> mode
 
 type frame' =
-  | F_aspar_ps   : e:exp -> frame'
-  | F_aspar_e    : ps:prins -> frame'
-  (*| F_assec_ps   : e:exp -> frame'
-  | F_assec_e    : v:value -> frame'*)
-  | F_box_e      : ps:prins -> frame'
-  | F_unbox      : frame'
-  | F_let        : x:varname -> e2:exp -> frame'
-  | F_app_e1     : e2:exp -> frame'
-  | F_app_e2     : v:value -> frame'
+  | F_aspar_ps: e:exp -> frame'
+  | F_aspar_e : ps:prins -> frame'
+  | F_box_e   : ps:prins -> frame'
+  | F_unbox   : frame'
+  | F_let     : x:varname -> e2:exp -> frame'
+  | F_app_e1  : e2:exp -> frame'
+  | F_app_e2  : v:value -> frame'
   
 type frame =
   | Frame: m:mode -> en:env -> f:frame'-> frame
@@ -142,9 +129,7 @@ val stack_target_inv: stack -> mode -> Tot bool
 let rec stack_target_inv s m = match s with
   | []                  -> true
   | (Frame m' _ f')::tl ->
-    let Mode _ ps = m in
-    let Mode _ ps' = m' in
-    (ps = ps' && stack_target_inv tl m)
+    (Mode.ps m = Mode.ps m' && stack_target_inv tl m)
 
 val stack_inv: stack -> mode -> level -> Tot bool
 let rec stack_inv s m l =
@@ -154,24 +139,8 @@ type config =
   | Conf: l:level -> m:mode{mode_inv m l} -> s:stack{stack_inv s m l}
           -> en:env -> t:term -> config
 
-
-val s_add: frame -> stack -> Tot stack
-let s_add = Cons
-
-val s_replace: frame -> s:stack{is_Cons s} -> Tot stack
-let s_replace f s = f::(Cons.tl s)
-
-val s_pop: c:config{is_Cons (Conf.s c)} -> Tot stack
-let s_pop c = Cons.tl (Conf.s c)
-
 val is_sframe: c:config -> f:(frame' -> Tot bool) -> Tot bool
 let is_sframe (Conf _ _ s _ _) f = is_Cons s && f (Frame.f (Cons.hd s))
-
-val pop_mode: c:config{is_Cons (Conf.s c)} -> Tot mode
-let pop_mode (Conf _ _ (fr::_) _ _) = Frame.m fr
-
-val pop_env: c:config{is_Cons (Conf.s c)} -> Tot env
-let pop_env (Conf _ _ (fr::_) _ _) = Frame.en fr
 
 val is_value: c:config -> Tot bool
 let is_value c = is_T_val (Conf.t c)
@@ -188,82 +157,96 @@ val c_value_ps: c:config{is_value_ps c} -> Tot prins
 let c_value_ps c = match c with
   | Conf _ _ _ _ (T_val (V_const (C_prins ps))) -> ps
 
-val is_redex: c:config -> Tot bool
-let is_redex c = is_T_red (Conf.t c)
-
-val is_exp: c:config -> Tot bool
-let is_exp c = is_T_exp (Conf.t c) 
-
-val pf_aspar_ps: c:config{is_sframe c is_F_aspar_ps} -> Tot exp
-let pf_aspar_ps (Conf _ _ ((Frame _ _ (F_aspar_ps e))::_) _ _) = e
-
-(*val pf_assec_ps: c:config{is_sframe c is_F_assec_ps} -> Tot exp
-let pf_assec_ps (Conf _ ((Frame _ _ (F_assec_ps e))::_) _ _) = e*)
-
-val pf_let: c:config{is_sframe c is_F_let} -> Tot (varname * exp)
-let pf_let (Conf _ _ ((Frame _ _ (F_let x e2))::_) _ _) = x, e2
-
-val pf_app_e1: c:config{is_sframe c is_F_app_e1} -> Tot exp
-let pf_app_e1 (Conf _ _ ((Frame _ _ (F_app_e1 e2))::_) _ _) = e2
-
-val pf_aspar_e: c:config{is_sframe c is_F_aspar_e} -> Tot prins
-let pf_aspar_e (Conf _ _ ((Frame _ _ (F_aspar_e ps))::_) _ _) = ps
-
-(*val pf_assec_e: c:config{is_sframe c is_F_assec_e} -> Tot value
-let pf_assec_e (Conf _ ((Frame _ _ (F_assec_e v))::_) _ _) = v*)
-
-val pf_box_e: c:config{is_sframe c is_F_box_e} -> Tot prins
-let pf_box_e (Conf _ _ ((Frame _ _ (F_box_e ps))::_) _ _) = ps
-
-val pf_app_e2: c:config{is_sframe c is_F_app_e2} -> Tot value
-let pf_app_e2 (Conf _ _ ((Frame _ _ (F_app_e2 v))::_) _ _) = v
-
 type is_easpar (c:config) =
   is_T_exp (Conf.t c) /\ is_E_aspar (Exp.e (T_exp.e (Conf.t c)))
-val pe_aspar: c:config{is_easpar c} -> Tot (exp * exp)
-let pe_aspar (Conf _ _ _ _ (T_exp (Exp (E_aspar e1 e2) _))) = e1, e2
-
-(*val pe_assec: c:config{is_E_assec (Exp.e (Conf.e c))} -> Tot (exp * exp)
-let pe_assec (Conf _ _ _ (Exp (E_assec e1 e2) _)) = e1, e2*)
 
 type is_eapp (c:config) =
   is_T_exp (Conf.t c) /\ is_E_app (Exp.e (T_exp.e (Conf.t c)))
-val pe_app: c:config{is_eapp c} -> Tot (exp * exp)
-let pe_app (Conf _ _ _ _ (T_exp (Exp (E_app e1 e2) _))) = (e1, e2)
 
 type is_eabs (c:config) =
   is_T_exp (Conf.t c) /\ is_E_abs (Exp.e (T_exp.e (Conf.t c)))
-val pe_abs: c:config{is_eabs c} -> Tot (varname * exp)
-let pe_abs (Conf _ _ _ _ (T_exp (Exp (E_abs x e) _))) = (x, e)
 
 type is_elet (c:config) =
   is_T_exp (Conf.t c) /\ is_E_let (Exp.e (T_exp.e (Conf.t c)))
-val pe_let: c:config{is_elet c} -> Tot (Tuple3 varname exp exp)
-let pe_let (Conf _ _ _ _ (T_exp (Exp (E_let x e1 e2) _))) = MkTuple3 x e1 e2
 
 type is_evar (c:config) =
   is_T_exp (Conf.t c) /\ is_E_var (Exp.e (T_exp.e (Conf.t c)))
-val pe_var: c:config{is_evar c} -> Tot varname
-let pe_var (Conf _ _ _ _ (T_exp (Exp (E_var x) _))) = x
 
 type is_econst (c:config) =
   is_T_exp (Conf.t c) /\ is_E_const (Exp.e (T_exp.e (Conf.t c)))
-val pe_const: c:config{is_econst c} -> Tot const
-let pe_const (Conf _ _ _ _ (T_exp (Exp (E_const c) _))) = c
 
 type is_eunbox (c:config) =
   is_T_exp (Conf.t c) /\ is_E_unbox (Exp.e (T_exp.e (Conf.t c)))
-val pe_unbox: c:config{is_eunbox c} -> Tot exp
-let pe_unbox (Conf _ _ _ _ (T_exp (Exp (E_unbox e) _))) = e
 
 val src: level -> Tot bool
 let src = is_Source
 
-val tgt: level -> Tot bool
-let tgt = is_Target
-
 (* pre returns comp, for src it's never Skip *)
 type comp = | Do | Skip | NA
+
+val step_aspar_e1: c:config{is_easpar c} -> Tot config
+let step_aspar_e1 (Conf l m s en (T_exp (Exp (E_aspar e1 e2) _))) =
+  Conf l m ((Frame m en (F_aspar_ps e2))::s) en (T_exp e1)
+  
+val step_unbox_e: c:config{is_eunbox c} -> Tot config
+let step_unbox_e (Conf l m s en (T_exp (Exp (E_unbox e) _))) =
+  Conf l m ((Frame m en F_unbox)::s) en (T_exp e)
+
+val step_const: c:config{is_econst c} -> Tot config
+let step_const (Conf l m s en (T_exp (Exp (E_const c) _))) =
+  Conf l m s en (T_val (V_const c))
+
+val step_var: c:config{is_evar c} -> Tot config
+let step_var (Conf l m s en (T_exp (Exp (E_var x) _))) =
+  Conf l m s en (T_val (en x))
+
+val step_let_e1: c:config{is_elet c} -> Tot config
+let step_let_e1 (Conf l m s en (T_exp (Exp (E_let x e1 e2) _))) =
+  Conf l m ((Frame m en (F_let x e2))::s) en (T_exp e1)
+
+val step_abs: c:config{is_eabs c} -> Tot config
+let step_abs (Conf l m s en (T_exp (Exp (E_abs x e) _))) =
+  Conf l m s en (T_val (V_clos en x e))
+
+val step_app_e1: c:config{is_eapp c} -> Tot config
+let step_app_e1 (Conf l m s en (T_exp (Exp (E_app e1 e2) _))) =
+  Conf l m ((Frame m en (F_app_e1 e2))::s) en (T_exp e1)
+
+val step_aspar_e2: c:config{is_value_ps c /\ is_sframe c is_F_aspar_ps}
+                   -> Tot config
+let step_aspar_e2 (Conf l _ ((Frame m en (F_aspar_ps e))::s) _
+                        (T_val (V_const (C_prins ps)))) =
+  Conf l m ((Frame m en (F_aspar_e ps))::s) en (T_exp e)
+
+val step_app_e2: c:config{is_value c /\ is_sframe c is_F_app_e1}
+                 -> Tot config
+let step_app_e2 (Conf l _ ((Frame m en (F_app_e1 e2))::s) _ (T_val v)) =
+  Conf l m ((Frame m en (F_app_e2 v))::s) en (T_exp e2)
+  
+val step_aspar_red: c:config{is_value c /\ is_sframe c is_F_aspar_e}
+                    -> Tot config
+let step_aspar_red (Conf l _ ((Frame m en (F_aspar_e ps))::s) _ (T_val v)) =
+  Conf l m s en (T_red (R_aspar ps v))
+
+val step_box_red: c:config{is_value c /\ is_sframe c is_F_box_e}
+                  -> Tot config
+let step_box_red (Conf l _ ((Frame m en (F_box_e ps))::s) _ (T_val v)) =
+  Conf l m s en (T_red (R_box ps v))
+
+val step_unbox_red: c:config{is_value c /\ is_sframe c is_F_unbox}
+                  -> Tot config
+let step_unbox_red (Conf l _ ((Frame m en F_unbox)::s) _ (T_val v)) =
+  Conf l m s en (T_red (R_unbox v))
+
+val step_let_red: c:config{is_value c /\ is_sframe c is_F_let}
+                  -> Tot config
+let step_let_red (Conf l _ ((Frame m en (F_let x e2))::s) _ (T_val v)) =
+  Conf l m s en (T_red (R_let x v e2))
+  
+val step_app_red: c:config{is_value c /\ is_sframe c is_F_app_e2}
+                  -> Tot config
+let step_app_red (Conf l _ ((Frame m en (F_app_e2 v1))::s) _ (T_val v2)) =
+  Conf l m s en (T_red (R_app v1 v2))
 
 val pre_aspar: config -> Tot comp
 let pre_aspar c = match c with
@@ -279,7 +262,7 @@ val step_aspar: c:config{not (pre_aspar c = NA)} -> Tot config
 let step_aspar c = match c with
   | Conf l m s en' (T_red (R_aspar ps (V_clos en x e))) ->
     let m'  = if src l then Mode Par ps else m in
-    let s'  = s_add (Frame m en' (F_box_e ps)) s in
+    let s'  = (Frame m en' (F_box_e ps))::s in
     
     (*
      * for parties not in ps, the choice of empty_env is arbitrary
@@ -294,24 +277,6 @@ let step_aspar c = match c with
     in
 
     Conf l m' s' en' t'
-
-(*val pre_assec: c:config -> Tot bool
-let pre_assec c = match c with
- | Conf (Mode _ ps1) _ _
-        (Exp (E_assec (Exp (E_value (V_const (C_prins ps2))) _)
-                      (Exp (E_value (V_clos _ _ _)) _)) _)
-        
-        -> ps1 = ps2
- 
- | _ -> false
-
-val pe_assec_beta: c:config{pre_assec c} -> Tot (Tuple4 prins env varname exp)
-let pe_assec_beta c = match c with
- | Conf _ _ _
-        (Exp (E_assec (Exp (E_value (V_const (C_prins ps))) _)
-                      (Exp (E_value (V_clos en x e)) _)) _)
-        
-        -> MkTuple4 ps en x e*)
 
 val pre_box: config -> Tot comp
 let pre_box c = match c with
@@ -358,216 +323,84 @@ let step_app c = match c with
   | Conf l m s _ (T_red (R_app (V_clos en x e) v)) ->
     Conf l m s (update_env en x v) (T_exp e)
 
-(* M; S; E; e --> M'; S'; E'; e' (common steps for source and target) *)
 type cstep: config -> config -> Type =
 
-  (* M; S; E; aspar e1 do e2 --> M; (M; E; aspar <> do e2)::S; E; e1*)
-
   | C_aspar_ps:
-    c:config{is_easpar c}
-    -> c':config{c' = Conf (Conf.l c) (Conf.m c)
-                           (s_add (Frame (Conf.m c) (Conf.en c)
-                                         (F_aspar_ps (snd (pe_aspar c))))
-                                  (Conf.s c))
-                           (Conf.en c) (T_exp(fst (pe_aspar c)))}
+    c:config{is_easpar c} -> c':config{c' = step_aspar_e1 c}
     -> cstep c c'
-
-  (* M; S; E; unbox e --> M; (M; E; unbox <>)::S; E; e *)
 
   | C_unbox:
-    c:config{is_eunbox c}
-    -> c':config{c' = Conf (Conf.l c)(Conf.m c)
-                           (s_add (Frame (Conf.m c) (Conf.en c) F_unbox)
-                                  (Conf.s c))
-                           (Conf.en c) (T_exp (pe_unbox c))}
+    c:config{is_eunbox c} -> c':config{c' = step_unbox_e c}
     -> cstep c c'
-
-  (* M; S; E; c --> M; S; E; c *)
 
   | C_const:
-    c:config{is_econst c}
-    -> c':config{c' = Conf (Conf.l c) (Conf.m c) (Conf.s c) (Conf.en c)
-                           (T_val (V_const (pe_const c)))}
+    c:config{is_econst c} -> c':config{c' = step_const c}
     -> cstep c c'
-
-  (* M; S; E; x --> M; S; E; E[x] *)
 
   | C_var:
-    c:config{is_evar c}
-    -> c':config{c' = Conf (Conf.l c) (Conf.m c) (Conf.s c) (Conf.en c)
-                           (T_val ((Conf.en c) (pe_var c)))}
+    c:config{is_evar c} -> c':config{c' = step_var c}
     -> cstep c c'
-
-  (* M; S; E; let x = e1 in e2 --> M; (M; E; let x = <> in e2)::S; E; e1  *)
 
   | C_let_e1:
-    c:config{is_elet c}
-    -> c':config{c' = Conf (Conf.l c) (Conf.m c)
-                           (s_add (Frame (Conf.m c) (Conf.en c)
-                                         (F_let (MkTuple3._1 (pe_let c))
-                                                (MkTuple3._3 (pe_let c))))
-                                  (Conf.s c)
-                           )
-                           (Conf.en c) (T_exp (MkTuple3._2 (pe_let c)))}
+    c:config{is_elet c} -> c':config{c' = step_let_e1 c}
     -> cstep c c'
-
-  (* M; S; E; fun x -> e --> M; S; E; clos(E, fun x -> e) *)
 
   | C_abs:
-    c:config{is_eabs c}
-    -> c':config{c' = Conf (Conf.l c) (Conf.m c) (Conf.s c) (Conf.en c)
-                           (T_val (V_clos (Conf.en c)
-                                          (fst (pe_abs c))
-                                          (snd (pe_abs c))))}
+    c:config{is_eabs c} -> c':config{c' = step_abs c}
     -> cstep c c'
-
-  (* M; S; E; e1 e2 --> M; (M; E; <> e2)::s; E; e1 *)
 
   | C_app_e1:
-    c:config{is_eapp c}
-    -> c':config{c' = Conf (Conf.l c) (Conf.m c)
-                           (s_add  (Frame (Conf.m c) (Conf.en c)
-                                          (F_app_e1 (snd (pe_app c))))
-                                   (Conf.s c)
-                           )
-                           (Conf.en c) (T_exp (fst (pe_app c)))}
+    c:config{is_eapp c} -> c':config{c' = step_app_e1 c}
     -> cstep c c'
-
-  (* M; (M'; E'; aspar <> do e)::S; E; v --> M'; (M'; E'; aspar v do <>)::s; E'; e *)
 
   | C_aspar_e:
     c:config{is_value_ps c /\ is_sframe c is_F_aspar_ps}
-    -> c':config{c' = Conf (Conf.l c) (pop_mode c)
-                           (s_replace (Frame (pop_mode c) (pop_env c)
-                                             (F_aspar_e (c_value_ps c)))
-                                      (Conf.s c))
-                           (pop_env c) (T_exp (pf_aspar_ps c))}
+    -> c':config{c' = step_aspar_e2 c}
     -> cstep c c'
-
-  (* M; (M'; E'; <> e)::S; E; v --> M'; (M'; E'; v <>)::S; E'; e *)
 
   | C_app_e2:
     c:config{is_value c /\ is_sframe c is_F_app_e1}
-    -> c':config{c' = Conf (Conf.l c) (pop_mode c)
-                           (s_replace (Frame (pop_mode c) (pop_env c)
-                                             (F_app_e2 (c_value c)))
-                                      (Conf.s c))
-                           (pop_env c) (T_exp (pf_app_e1 c))}
+    -> c':config{c' = step_app_e2 c}
     -> cstep c c'
 
-  (* _; (M'; E'; aspar v1 do <>))::S; _; v2 --> M'; S; E'; aspar v1 do v2  *)  
-  
-  | C_aspar_rec:
+  | C_aspar_red:
     c:config{is_value c /\ is_sframe c is_F_aspar_e}
-    -> c':config{c' = Conf (Conf.l c) (pop_mode c) (s_pop c) (pop_env c)
-                           (T_red (R_aspar (pf_aspar_e c) (c_value c)))}
+    -> c':config{c' = step_aspar_red c}
     -> cstep c c'
 
-  (* _; (M'; E'; box v1 <>))::S; _; v2 --> M'; S; E'; box v1 v2  *)
-  
-  | C_box_rec:
+  | C_box_red:
     c:config{is_value c /\ is_sframe c is_F_box_e}
-    -> c':config{c' = Conf (Conf.l c) (pop_mode c) (s_pop c) (pop_env c)
-                           (T_red (R_box (pf_box_e c) (c_value c)))}
+    -> c':config{c' = step_box_red c}
     -> cstep c c'
 
-  (* _; (M; E; unbox <>)::S; _; v --> M; S; E; unbox v*)
-
-  | C_unbox_rec:
+  | C_unbox_red:
     c:config{is_value c /\ is_sframe c is_F_unbox}
-    -> c':config{c' = Conf (Conf.l c) (pop_mode c) (s_pop c) (pop_env c)
-                           (T_red (R_unbox (c_value c)))}
+    -> c':config{c' = step_unbox_red c}
     -> cstep c c'
 
-  (* _; (M; E; let x = <> in e)::S; _; v --> M; S; E; let x = v in e  *)
-
-  | C_let_rec:
+  | C_let_red:
     c:config{is_value c /\ is_sframe c is_F_let}
-    -> c':config{c' = Conf (Conf.l c) (pop_mode c) (s_pop c) (pop_env c)
-                           (T_red (R_let (fst (pf_let c)) (c_value c)
-                                         (snd (pf_let c))))}
+    -> c':config{c' = step_let_red c}
     -> cstep c c'
 
-  (* _; (M; E; v1 <>)::S; _; v2 --> M; S; E; v1 v2 *)
-  | C_app_rec:
+  | C_app_red:
     c:config{is_value c /\ is_sframe c is_F_app_e2}
-    -> c':config{c' = Conf (Conf.l c) (pop_mode c) (s_pop c) (pop_env c)
-                           (T_red (R_app (pf_app_e2 c) (c_value c)))}
+    -> c':config{c' = step_app_red c}
     -> cstep c c'
 
-  (* M; S; E; let x = v1 in e2 --> M; S; E[x -> v]; e2 *)
-  
   | C_let_beta:
     c:config{is_let_redex c} -> c':config{c' = step_let c} -> cstep c c'
     
-  (* M; S; _; (E, fun x -> e) v --> M; S; E[x -> v]; e *)
   | C_app_beta:
     c:config{is_app_redex c} -> c':config{c' = step_app c} -> cstep c c'
 
-  (* M; S; E; assec e1 do e2 --> M; (M; E; assec <> do e2)::S; E; e1 *)
-
-  (*| S_assec_ps:
-    c:config{is_E_assec (Exp.e (Conf.e c)) /\ not (is_reduced c)}
-    -> c':config{c' = Conf (Conf.m c)
-                           (s_add (Frame (Conf.m c) (Conf.en c)
-                                         (F_assec_ps (snd (pe_assec c))))
-                                  (Conf.s c))
-                           (Conf.en c) (fst (pe_assec c))}
-    -> sstep c c'*)
-
-  (* M; (M'; E'; assec <> do e)::S; E; v --> M'; (M'; E'; assec v do <>)::s; E'; e *)
-
-  (*| S_assec_e:
-    c:config{is_value c /\ is_sframe c is_F_assec_ps}
-    -> c':config{c' = Conf (pop_mode c) (s_replace (Frame (pop_mode c) (pop_env c)
-                                                          (F_assec_e (pe_value c)))
-                                                   (Conf.s c))
-                           (pop_env c) (pf_assec_ps c)}
-    -> sstep c c'*)
-
-  (* _; (M'; E'; assec v1 do <>))::S; _; v2 --> M'; S; E'; assec v1 do v2  *)
-  
-  (*| S_assec_rec:
-    c:config{is_value c /\ is_sframe c is_F_assec_e}
-    -> c':config{c' = Conf (pop_mode c) (s_pop c) (pop_env c)
-                           (e_assec (e_value (pf_assec_e c))
-                                    (e_value (pe_value c)))}
-    -> sstep c c'*)
-    
-  (* M; S; _; aspar ps do clos(E, fun x -> e)  (when M is Par(ps1) /\ sub ps ps1
-     -->
-     Par(ps); (Par(ps); E; Box ps <>)::S; E[x -> ()]; e
-  *)
   | C_aspar_beta:
     c:config{not (pre_aspar c = NA)} -> c':config{c' = step_aspar c}
     -> cstep c c'
 
-  (* M; S; _; assec ps do clos(E, fun x -> e)  (when ps = M.ps)
-     -->
-     Sec(ps); S; E[x -> ()]; e
-  *)
-  (*| S_assec_beta:
-    c:config{pre_assec c}
-    -> c':config{c' = Conf (Mode Sec (MkTuple4._1 (pe_assec_beta c))) (Conf.s c)
-                           (update_env (MkTuple4._2 (pe_assec_beta c))
-                                       (MkTuple4._3 (pe_assec_beta c))
-                                       (V_const C_unit))
-                           (MkTuple4._4 (pe_assec_beta c))}
-    -> sstep c c'*)
-
-  (* M; S; E; box ps v (when is_Par M /\ sub ps M.ps)
-     -->
-     M; S; E; Box ps v
-  *)
-
   | C_box_beta:
     c:config{pre_box c = Do} -> c':config{c' = step_box c} -> cstep c c'
 
-  (* M; S; E; unbox (Box ps v) (when isPar M ==> sub M.ps ps /\
-                                     isSec M ==> sub ps M.ps)
-     -->
-     M; S; E; v                                   
-  *)
   | C_unbox_beta:
     c:config{pre_unbox c = Do} -> c':config{c' = step_unbox c}
     -> cstep c c'
@@ -577,18 +410,20 @@ type cstep: config -> config -> Type =
 assume val preceds_axiom: en:env -> x:varname -> Lemma (ensures (en x << en))
 
 val slice_v : prin -> v:value -> Tot value (decreases %[v])
-val slice_en: prin -> en:env -> varname -> Tot value (decreases %[en])
+val slice_en: prin -> en:env -> Tot (varname -> Tot value) (decreases %[en])
 
-// (fun y -> preceds_axiom en y; slice_v p (en y)) x e
 let rec slice_v p v =
   match v with
+    | V_const _     -> v
     | V_box ps v'   ->
       let v'' = if mem p ps then slice_v p v' else V_emp in
       V_box ps v''
     | V_clos en x e -> V_clos (slice_en p en) x e
-    | _             -> v
+    | V_emp         -> v
 
-and slice_en p en x = preceds_axiom en x; slice_v p (en x)// fun x -> slice_v p (en x)
+and slice_en p en =
+  let _ = () in
+  fun x -> preceds_axiom en x; slice_v p (en x)
 
 assume val slice_emp_en: p:prin
                          -> Lemma (requires (True))
@@ -608,11 +443,15 @@ let slice_r p r = match r with
   | R_let x v1 e2 -> R_let x (slice_v p v1) e2
   | R_app v1 v2   -> R_app (slice_v p v1) (slice_v p v2)
 
-(* only frame' with values need to be sliced *)
 val slice_f': p:prin -> frame' -> Tot frame'
 let slice_f' p f = match f with
-  | F_app_e2  v -> F_app_e2  (slice_v p v)
-  | _           -> f
+  | F_aspar_ps _ -> f
+  | F_aspar_e  _ -> f
+  | F_box_e    _ -> f
+  | F_unbox      -> f
+  | F_let    _ _ -> f
+  | F_app_e1   _ -> f
+  | F_app_e2   v -> F_app_e2  (slice_v p v)
 
 val slice_f: p:prin -> f:frame{Mode.m (Frame.m f) = Par /\
                                mem p (Mode.ps (Frame.m f))}
@@ -659,15 +498,6 @@ let env_upd_slice_lemma p en x v =
   cut (FEq (slice_en p (update_env en x v))
       (update_env (slice_en p en) x (slice_v p v)))
 
-
-(* TODO: FIXME: bug#259 *)
-val v_clos_slice_lemma: #en:env -> #x:varname -> #e:exp
-                        -> p:prin -> v:value{v = V_clos en x e}
-                        -> Lemma (requires (True))
-                                 (ensures  (slice_v p v = V_clos (slice_en p en) x e))
-let v_clos_slice_lemma #en #x #e p v = admit ()
-
-
 val cstep_lemma: #c:sconfig -> #c':sconfig -> h:cstep c c' -> p:prin
                  -> Tot (cor (u:unit{slice_c p c = slice_c p c'})
                              (cstep (slice_c p c) (slice_c p c')))
@@ -690,8 +520,6 @@ let cstep_lemma #c #c' h p = match h with
   | C_abs (Conf _ m _ en _) _ ->
     if not (mem p (Mode.ps m)) then IntroL ()
     else
-      let T_exp (Exp (E_abs x e) _) = Conf.t c in
-      v_clos_slice_lemma #en #x #e p (V_clos en x e);
       IntroR (C_abs (slice_c p c) (slice_c p c'))
   | C_app_e1 (Conf _ m _ _ _) _ ->
     if not (mem p (Mode.ps m)) then IntroL ()
@@ -702,24 +530,24 @@ let cstep_lemma #c #c' h p = match h with
   | C_app_e2 (Conf _ m _ _ _) _ ->
     if not (mem p (Mode.ps m)) then IntroL ()
     else IntroR (C_app_e2 (slice_c p c) (slice_c p c'))
-  | C_aspar_rec (Conf _ m _ _ _) _ ->
+  | C_aspar_red (Conf _ m _ _ _) _ ->
     if not (mem p (Mode.ps m)) then IntroL ()
-    else IntroR (C_aspar_rec (slice_c p c) (slice_c p c'))
-  | C_box_rec (Conf _ m s _ _) _ ->
+    else IntroR (C_aspar_red (slice_c p c) (slice_c p c'))
+  | C_box_red (Conf _ m s _ _) _ ->
     if mem p (Mode.ps m) then
-      IntroR (C_box_rec (slice_c p c) (slice_c p c'))
+      IntroR (C_box_red (slice_c p c) (slice_c p c'))
     else if mem p (Mode.ps (Frame.m (Cons.hd s))) then
-      IntroR (C_box_rec (slice_c p c) (slice_c p c'))
+      IntroR (C_box_red (slice_c p c) (slice_c p c'))
     else IntroL ()
-  | C_unbox_rec (Conf _ m _ _ _) _ ->
+  | C_unbox_red (Conf _ m _ _ _) _ ->
     if not (mem p (Mode.ps m)) then IntroL ()
-    else IntroR (C_unbox_rec (slice_c p c) (slice_c p c'))
-  | C_let_rec (Conf _ m _ _ _) _ ->
+    else IntroR (C_unbox_red (slice_c p c) (slice_c p c'))
+  | C_let_red (Conf _ m _ _ _) _ ->
     if not (mem p (Mode.ps m)) then IntroL ()
-    else IntroR (C_let_rec (slice_c p c) (slice_c p c'))
-  | C_app_rec (Conf _ m _ _ _) _ ->
+    else IntroR (C_let_red (slice_c p c) (slice_c p c'))
+  | C_app_red (Conf _ m _ _ _) _ ->
     if not (mem p (Mode.ps m)) then IntroL ()
-    else IntroR (C_app_rec (slice_c p c) (slice_c p c'))
+    else IntroR (C_app_red (slice_c p c) (slice_c p c'))
   | C_let_beta (Conf _ m _ _ _) _ ->
     if not (mem p (Mode.ps m)) then IntroL ()
     else
@@ -729,15 +557,13 @@ let cstep_lemma #c #c' h p = match h with
   | C_app_beta (Conf _ m _ _ _) _ ->
     if not (mem p (Mode.ps m)) then IntroL ()
     else
-      let T_red (R_app (V_clos en x e) v) = Conf.t c in
-      v_clos_slice_lemma #en #x #e p (V_clos en x e);
+      let T_red (R_app (V_clos en x _) v) = Conf.t c in
       env_upd_slice_lemma p en x v;
       IntroR (C_app_beta (slice_c p c) (slice_c p c'))
   | C_aspar_beta (Conf _ m _ _ _) _ ->
     if not (mem p (Mode.ps m)) then IntroL ()
     else
-      let T_red (R_aspar _ (V_clos en x e)) = Conf.t c in
-      v_clos_slice_lemma #en #x #e p (V_clos en x e);
+      let T_red (R_aspar _ (V_clos en x _)) = Conf.t c in
       env_upd_slice_lemma p en x (V_const (C_unit));
       IntroR (C_aspar_beta (slice_c p c) (slice_c p c'))
   | C_box_beta (Conf _ m _ _ _) _ ->
